---
title: 
description: 
aliases: []
tags: []
created: 2024-12-04T21:50:46
modified: 2025-02-09T15:53:46
permalink:
---

worked example: Find the derivative of $f(x)=4x^2$
$f'(x)=4\cdot \dfrac{d}{dx}[x^2]$
$f'(x)=4\cdot 2x$

worked example: Find the derivative of $f(x)=2x^7$
$f'(x)=(7)(2)x^{7-1}=14x^6$

worked example: Find the derivative of $f(x)=4x^2+5$
$f'(x)=\dfrac{d}{dx}[4x^2]+\dfrac{d}{dx}[5]$
$f'(x)=8x+0$

worked example: Find the derivative of $f(x)=4x^2+5x$
$f'(x)=\dfrac{d}{dx}[4x^2]+(5)\dfrac{d}{dx}[x]$
$f'(x)=8x+(5)(1)$

worked example: Find the derivative of $f(x)=4x^2+5x+6$
$f'(x)=\dfrac{d}{dx}[4x^2]+(5)\dfrac{d}{dx}[x]+\dfrac{d}{dx}[6]$
$f'(x)=8x+5+0$

worked example: Find $f'(1)$ for $f(x)=5x^3+2x+5$
$f'(x)=15x^2+2$
$f'(1)=17$

worked example: Differentiate $f(x)=x^{-\dfrac{1}{2}}$

$f'(x)=-\dfrac{1}{2}\cdot x^{-\dfrac{3}{2}}$
$f'(x)=-\dfrac{1}{2}\cdot \dfrac{1}{(\sqrt{x})^3}$


worked example: Differentiate $f(x)=\dfrac{1}{2x}+x^3$

$f'(x)=(\dfrac{1}{2})\dfrac{d}{dx}[x]+\dfrac{d}{dx}[x^2]$
$f'(x)=\dfrac{1}{2}+2x$


worked example: Differentiate $f(x)=\dfrac{1}{x}+\dfrac{1}{\sqrt{x}}$

$f(x)=x^{-1}+x^{-\dfrac{1}{2}}$

$f'(x)=(-1)x^{-2}+(-\dfrac{1}{2})x^{-\dfrac{3}{2}}$



worked example: Differentiate $f(x)=2x^2-\dfrac{1}{x}$
$f(x)=2x^2-x^{-1}$
$f'(x)=4x+\dfrac{1}{x^2}$


worked example: Differentiate $f(x)=\dfrac{x-3}{2x^2-7x+3}$ by factorizing first

$f(x)=\dfrac{x-3}{2x^2-6x-x+3}$

$f(x)=\dfrac{x-3}{2x(x-3)+(-1)(x-3)}$

$f(x)=\dfrac{x-3}{(2x-1)(x-3)}$

$f(x)=\dfrac{1}{2x-1}$

$f'(x)=(-1)(2x-1)^{-2}$

$f'(x)=\dfrac{-1}{(2x-1)^2}$

worked example: Differentiate $f(x)=\dfrac{x-2}{3x^2-5x-2}$ by factorizing first

$f(x)=\dfrac{x-2}{3x^2-6x+x-2}$

$f(x)=\dfrac{x-2}{3x(x-2)+1(x-2)}$

$f(x)=\dfrac{x-2}{(3x+1)(x-2)}$

$f(x)=\dfrac{1}{3x+1}$

$f'(x)=(-1)(3x+1)^{-2}$

$f'(x)=\dfrac{-1}{(3x+1)^2}$


worked example: Differentiate $f(x)=e^{5x}+e^7-e^{-x}$

$f'(x)=5e^{5x}+0+e^{-x}$


worked example: Differentiate $f(x)=-\dfrac{1}{2\sqrt{x}}$

$f(x)=-\dfrac{1}{2}x^{-\frac{1}{2}}$

$f'(x)=\dfrac{1}{4}x^{-\frac{3}{2}}$

worked example: Differentiate $f(x)=\dfrac{e^{2x}-e^x+1}{e^x}$

$f(x)=\dfrac{e^{2x}}{e^x}-1+\dfrac{1}{e^x}$

$f(x)=e^x-1+\dfrac{1}{e^x}$

$f(x)=e^x-1+e^{-x}$

$f'(x)=e^x-e^{-x}$


worked example: Differentiate $f(x)=\dfrac{1}{x^3}-\dfrac{2}{x^2}$

$f(x)=x^{-3}-2\cdot x^{-2}$
$f'(x)=-3x^{-4}+4x^{-3}$
