---
title: 
description: 
aliases: []
tags: []
created: 2024-11-19T21:16:10
modified: 2025-03-09T11:10:01
permalink:
---

Exponentiation is an operation involving two numbers - the base and the exponent.

The division was a lie. Just like how subtraction was a lie. Because $2\div 7=2\cdot7^{-1}$.
The square root was also a lie. It's just an exponent. Because $\sqrt[2]{7}=7^{\dfrac{1}{2}}$ and $\sqrt[3]{7}=7^{\dfrac{1}{3}}$.

Exponent identities.

$a^0=1$

$a^1=a$

$(a \cdot b)^{c}=a^{c} \cdot b^{c}$

$a^{b}\cdot a^{c} = a^{b+c}$

$(a^{b})^c=a^{bc}$

$\dfrac{a^{b}}{a^{c}} = a^{b-c}$

$a^{-b}=\dfrac{1}{a^{b}}$

$a^{\dfrac{1}{b}}=\sqrt[b]{a}$

$\dfrac{a^c}{b^c}=\left(\dfrac{a}{b}\right)^c$

```anki
id: 1741511531597
---
==$\dfrac{a^c}{b^c}$==  = ==$\left(\dfrac{a}{b}\right)^c$==
```

$(a+b)^2=a^2+2ab+b^2$

$a^2-b^2=(a+b)(a-b)$

$(a+b)^3=a^3+3ab^2+3a^2b+b^3$

$a^3+b^3=(a+b)(a^2-ab+b^2)$
 
From the rules above, we can derive more.

$\left(\dfrac{a}{b}\right)^c = a^c \cdot b^{-c}$


$\left(\dfrac{a}{b}\right)^c = \dfrac{(a)^c}{(b)^c} = (a)^c\cdot\left(\dfrac{1}b\right)^c = a^c \cdot b^{-c}$

$a^2+ba=\left(a+\dfrac{b}{2}\right)^2-\left(\dfrac{b}{2}\right)^2$

$a^2+ba+c=a\left(b-(-\dfrac{b}{2a})\right)^2+\left(c-\dfrac{b^2}{4a}\right)$
