---
title: 
description: 
aliases: []
tags: []
created: 2025-01-30T13:13:11
modified: 2025-02-09T15:53:45
permalink:
---


For a given function $f(x)$, transformations can change the graph.


This guide will focus on the simple transformations of a function - dilation, reflection and translation.


Firstly, think about a point, $(a,b)$ on the plane. After it undergoes all the transformations it wants, we end up with a point, $(a',b')$.

So essentially, two variables, we do things, and end up with two variables. This is a function with two inputs and two outputs - $t(a,b)=\{g(a,b),h(a,b)\}$


- Worked example: The point $(2,3)$ is transformed using the function $t(a,b)=\{ a+1, -2b \}$, Resulting in $(a',b')$. Find $(a',b')$.

Directly using the function, we see that $t(2,3)=\{3,-6\}$ and $(a',b')=(3,-6)$



- Worked example: The function $y=x^2$ is dilated by factor of 3 from the x-axis. Find the resulting image function, $y'$.

A dilation of 3 from the x-axis means $y'=3y$.

In the beginning we have $y=x^2$
In the end we have $y'=x'$

$x'=x$
$y'=3y$


So $y'=3x^2$



- Worked example: The function $y=3x^2$ is translated to the right by 7 units. Find the resulting image function, $y'$.

A translation to the right means $x'=x+7$

In the beginning we have $y=3x^2$
In the end we have $y'=x'$

$x'=x+7$
$y'=y$

So $y'=3x^2+7$


- Worked example: The function $y=x^2$ is translated upwards by 7 units. Then it is reflected across the x-axis. Find the resulting image function, $y'$.

A translation upwards means $y'=y+7$
A reflection in the x-axis means $y'=-y$

In the beginning we have $y=x^2$
In the end we have $y'=x'$

original
$y'=y$
translate
$y'=y+7$
reflect
$y'=-y-7$

So $y'=-x^2-7$


- Worked example: The function $y=x^2$ is translated to the left by 6 units. Then it is dilated by factor of $\dfrac{1}{3}$ in the y-axis. Find the resulting image function, $y'$.

A translation to the left means $x'=x-6$
A dilation in the y-axis means $x'=\dfrac{1}{3}x$

In the beginning we have $y=x^2$
In the end we have $y'=x'$

original
$x'=x$
translation
$x'=x-6$
dilation
$x'=\dfrac{1}{3}x-2$

So $y'=\dfrac{1}{3}x-2$



- Worked example: The function $y=x^2$ is translated 












- Worked example: State the sequence of transformations needed to transform $y=x^2$ into the image function $y'=2x^2+4x+2$

break down terms of $x$ - $2x^2+4x+2=2(x^2+2x+1)=2(x+1)^2$

original
$y=x^2$
dilation
$y=2x^2$
