---
title: 
description: 
aliases: []
tags: []
created: 2025-05-21T11:44:19
modified: 2025-05-28T14:22:08
permalink:
---

## For $f(x)=\sin(\dfrac{5x}{4})$, what is $f'(\dfrac{11\pi}{5})$?

$f'(x)=\cos(\dfrac{5x}{4})(\dfrac{5}{4})$
$f'(\dfrac{11\pi}{5})=\cos(\dfrac{11\pi}{4})(\dfrac{5}{4})$
$=(\dfrac{-\sqrt{2}}{2})(\dfrac{5}{4})$
$=\dfrac{-5\sqrt{2}}{8}$

## Find $f'(x)$ for $f(x)=\tan(3x+1)$.

$f'(x)=\sec^2(3x+1)(3)$

## Find $f'(x)$ for $f(x)=\dfrac{1}{(\cos(2x)+3)^3}$.

$\dfrac{d}{dx}\left[\dfrac{1}{f(x)}\right]=-\dfrac{f'(x)}{f(x)^2}$

$f'(x)=\dfrac{(-3)(\cos(2x)+3)^2(-\sin(2x)(2))}{(\cos(2x)+3)^6}$

$f'(x)=\dfrac{(6)(\cos(2x)+3)^2\sin(2x)}{(\cos(2x)+3)^6}$

$f'(x)=\dfrac{6(\sin(2x)}{(\cos(2x)+3)^4}$

## For $f(x)=x^2+e^x-2$, find the equation of the tangent to the graph when $x=0$.

$f'(x)=2x+e^x$
$m_T=f'(0)=1$

$f(0)=-1$
$y=mx+c$
$y=x-1$

## Find $f''(x)$ for $f(x)=x^2\cos(2x)$.

$f'(x)=(2x)(\cos(2x))+(x^2)(-\sin(2x)(2))$
$f''(x)=2\cos(2x)\cdot -4x\sin(2x))+(4x)(-\sin(2x)))(x^2)(-2\cos(2x))$
$f''(x)=$

## Find $f'(x)$ for $f(x)=2\tan(\tan(3x+1))$. >H<

$f'(x)=2\sec^2(\tan(3x+1)(\sec^2(3x+1)(3)))$

$f'(x)=\dfrac{2}{\cos^2(\dfrac{3\tan(3x+1)}{\cos^2(3x+1)})}$

## Consider the function $f(x)=\sin(2x)$. If P is the point (x,f(x)) and Q is the point (x+h,f(x+h)), $h\neq0$ . What is gradient of the secant PQ in terms of x and h?

$f'(x)=\lim\limits_{h\to0}\dfrac{f(x+h)-f(x)}{h}$.

$f'(x)=\lim\limits_{h\to0}\dfrac{\sin(2x+2h)-\sin(2x)}{h}$.

## For $f(x)=e^x(px^2+qx+r)$, the curve y=f(x) is such that the tangents at x=0 and x=1 are parallel to the x-axis. The point with coordinates (0,1) is on the curve. Find p,q and r.

$f'(0)=0$
$f'(1)=0$

$f(0)=1$

$f'(x)=(e^x)(px^2+qx+r)+(e^x)(2px+q)$
$f'(0)=r+q=0$
$f'(1)=3pe+2qe+re=0$
$f(0)=r=1$
$q=-1$
$3pe-2e+e=0$
$3p-1=0$
$p=\dfrac{1}{3}$

## For $f(x)=x\sin(x)$, find the tangent to the graph at $x=\dfrac{-5\pi}{2}$.

$f'(x)=\sin(x)+x\cos(x)$
$m_T=f'(\dfrac{-5\pi}{2})=-1$
$y-y_1=m(x-x_1)$

$f(\dfrac{-5\pi}{2})=\dfrac{5\pi}{2}$
$y-\dfrac{5\pi}{2}=-1(x+\dfrac{5\pi}{2})$
$y=-x$

## For $f(x)=x\sin(x)$, find $f'(\dfrac{11\pi}{4})$.

## For $f(x)=(\tan(x)+2)^2$, find $f'(x)$.

## For $f(x)=a \sqrt{3}\sin(x)+b\cos(x)$ where $a,b<0$, state the relationship between a and b if there is a local minimum at $x=\dfrac{\pi}{3}$.

$f'(x)=a\sqrt{3}\cos(x)-b\sin(x)$
$f'(\dfrac{\pi}{3})=0$
$0=a\sqrt{3}\cos(\dfrac{\pi}{3})-b\sin(\dfrac{\pi}{3})$
$0=\dfrac{\sqrt{3}}{2}a-\dfrac{\sqrt{3}}{2}b$
$a=b$

## For $f(x)=\cos(2x)+\sin(x)+x^2$, find $f''(x)$.

$f'(x)=-2\sin(2x)+\cos(x)+2x$
$f''(x)=-4\cos(x)-\sin(x)+2$

## The average rate of change of $f(x)=\log_2(\dfrac{x^3}{4})$ over the interval $2\leq x\leq4$ is:

rise over run

$\dfrac{f(4)-f(2)}{2}=\dfrac{4-1}{2}=\dfrac{3}{2}$

## The value of the gradient of curve $f(x)=\cos(x)\sin(x)$ at $x=\dfrac{\pi}{3}$ is:

$f'(x)=-\sin(x)\sin(x)+\cos(x)\cos(x)$
$f'(x)=-\sin^2(x)+\cos^2(x)$
$f'(\dfrac{\pi}{3})=\dfrac{-3}{4}+\dfrac{1}{4}=\dfrac{-1}{2}$

## For $f:[1,3]→\mathbb{R},f(x)=x^2+kx+4$, find the value(s) of k such that the absolute maximum of the function occurs when x=1.

There can be many absolute maximums.

We know that $f(1)\geq(3)$.

$k+5\geq3k+13$
$2k\leq-8$
$k\leq-4$

## Let f be a one-to-one differentiable function such that f(3)=7,f(7)=8,f′(3)=2 and f′(7)=3. The function g is differentiable and g(x)=f−1(x) for all x.  Find g′(7).

We know that $g(f(x))=x$
Take derivative of both sides
$g'(f(x))f'(x)=1$
Rearrange
$f'(x)=\dfrac{1}{g'(f(x))}$

In this case,

$g'(7)=\dfrac{1}{f'(g(7))}=\dfrac{1}{f'(3)}=\dfrac{1}{2}$
