---
title: 
description: 
aliases: []
tags: []
created: 2025-03-09T14:21:35
modified: 2025-03-17T20:27:18
permalink:
---

## What is $y=2x^2$ after dilation 2 in x axis?

$x,y\to x'=x, y'=2y$
$x=x', y=\dfrac{1}{2}y'$
$y=2x^2$
$\to$
$\dfrac{1}{2}y=2x^2$
$y=4x^2$

## $y=\dfrac{-3}{(2x-1)^2}+5$. Translate 1 right and 7 down. Then dilate $\dfrac{1}{2}$ from x axis and dilate 2 from y axis. Then reflect in y axis.

$x'=x,y'=y$
$\to$
$x'=x+1,y'=y-7$
$\to$
$x'=2(x+1),y'=\dfrac{1}{2}(y-7)$
$\to$
$x'=-2(x+1),y'=\dfrac{1}{2}(y-7)$
$x=\dfrac{x'}{-2}-1$
$y=2y'+7$

$y=\dfrac{-3}{(2x-1)^2}+5$
$\to$
$2y+7=\dfrac{-3}{(-x-3)^2}+5$
$2y+7=\dfrac{-3}{(-1(x+3))^2}+5$
$2y+7=\dfrac{-3}{(x+3)^2}+5$
$2y=\dfrac{-3}{(x+3)^2}-2$
$y=\dfrac{-3}{2(x+3)^2}-1$

## The graph of $y=2x$ is translated 1 right and 3 up, what is the resulting function?

$x,y \to x'=x+1, y'=y+3$
$x=x'-1,y=y'-3$
$y=2x$
$y'-3=2x'-2$
$\to$
$y=2x+1$

## The point $(9,11)$ lies on f. The graph is dilated by $\dfrac{1}{3}$ from the x axis and translated down 5 units. Find the image of the point.

$x,y \to x'=x, y'=\dfrac{1}{3}y-5$
$(9,11)\to(9,\dfrac{-4}{3})$

## $f(x)=(x-2)(x+4)$. If a horizontal translation in the form $y=f(x-k)$ is applied, what values of k will the function have 2 positive solutions?

The original function has roots at x=2 and x=-4. We will need a horizontal translation of more than 4 right.

$k>4$

## What is $y=3x^2+2$ after dilation of 3 from y axis?

$x,y\to x'=3x,y'=y$
$x=\dfrac{x'}{3}$
$y=3x^2+2$
$\to$
$y=\dfrac{x^2}{3}+2$

## What is $y=\sqrt{3x-9}$ after reflection in x axis, then dilation $\dfrac{1}{3}$ in y axis.

$x,y\to x'=\dfrac{1}{3}x,y'=-y$
$x=3x',y=-y'$
$y=\sqrt{3x-9}$
$\to$
$-y=\sqrt{3(3x)-9}$
$y=-\sqrt{9x-9}$

## The transformation $T(x,y)=(-2x+6, 3y-2)$ transforms a graph into $y=4x-12$. What is the pre-image?

$x,y\to x'=-2x+6,y'=3y-2$

$y'=4x'-12$
$\to$
$3y-2=4(-2x+6)-12$
$3y-2=-8x+24-12$
$3y=-8x+14$
$y=\dfrac{-8}{3}+\dfrac{14}{3}$

## The transformation $T(x,y)=(3x+2,-y+4)$ transforms a graph into $y=\dfrac{(x-3)^2}{6}+2$. What is the pre-image?

$x,y\to x'=3x+2,y'=-y+4$

$y'=\dfrac{(x'-3)^2}{6}+2$
$\to$
$-y+4=\dfrac{(3x+2-3)^2}{6}+2$
$-y=\dfrac{(3x-1)^2}{6}-2$
$y=\dfrac{-(3x-1)^2}{6}+2$

## What is $y=-\sqrt{1-x}+1$ after dilation 5 from y axis, then reflection in y axis, then translate 2 left and 8 up.

$x,y\to x'=-5x-2,y'=y+8$
$x=\dfrac{x'+2}{-5}$
$y=y'-8$

$y=-\sqrt{1-x}+1$
$\to$
$y-8=-\sqrt{1-\dfrac{x+2}{-5}}+1$
$y-8=-\sqrt{\dfrac{5}{5}+\dfrac{x+2}{5}}+1$
$y=-\sqrt{\dfrac{x+7}{5}}+9$

## What is $y=x^4+6x^2+9$ after translation 1 up, then reflection in y axis, then dilation 2 from x axis.

$x'=x,y'=y$
$\to$
$x'=x+1,y'=y$
$\to$
$x'=-(x+1),y'=y$
$\to$
$x'=-(x+1),y'=2y$

$x=-x'-1$
$y=\dfrac{y'}{2}$


$y=x^4+6x^2+9$
$\to$
$\dfrac{y}{2}=(-x-1)^4+6(-x-1)^2+9$
$y=2(x+1)^4+12(x+1)^2+18$
$y=2(x^4+4x^3+4x^2+1)+12(x^2+2x+1)+18$
$y=2x^4+8x^3+24x^2+32x+32$

## $f:[0,\infty)\to\mathbb{R},f(x)=x^3+x$. What is the range of the image function after reflection in x axis?

The original domain is $[0,\infty]$.

Find the original range.

$f'(x)=3x^2+1$, and we know that $x\geq0,$ meaning $f'(x)\geq 0$. The graph is strictly increasing.

$f(0)=0$

So the range is $[0,\infty)$.

After the reflection, the range is $(-\infty,0]$.

## The point $(-1,\dfrac{1}{2})$ lies on d. The graph is reflected in both axes , then translated 1 left. Find the image of the point.

$x,y\to x'=-x-1,y'=-y$

$(-1,\dfrac{1}{2})\to(0,-\dfrac{1}{2})$

## Describe the transformations that map $y=\dfrac{4}{(2x+1)^2}-6$ onto $y=\dfrac{10}{(x-1)^2}+3$.

$y'=\dfrac{10}{(x'-1)^2}+3$
$\dfrac{y'-3}{10}=\dfrac{1}{(x'-1)^2}$


$y=\dfrac{4}{(2x+1)^2}-6$

$y+6=\dfrac{4}{(2x+1)^2}$
$\dfrac{y+6}{4}=\dfrac{1}{(2x+1)^2}$
$\to$
$\dfrac{y'-3}{10}=\dfrac{1}{(x'-1)^2}$

$\dfrac{y+6}{4}=\dfrac{y'-3}{10}$
$10y+60=4y'-12$
$y'=\dfrac{10y+72}{4}$
$y'=\dfrac{5}{2}y+18$

$\dfrac{1}{(2x+1)^2}=\dfrac{1}{(x'-1)^2}$
$2x+1=x'-1$
$x'=2x+2$

- Dilate 2 from y axis.
- Dilate $\dfrac{5}{2}$ from x axis.
- Translate 2 right and 18 up.

## $f(x)=(x-3)^3+3$. If vertical translation of $k$ is applied, what values of $k$ will the x-intercept be at $(3,0)$?

We want to solve the equation $0=(3-3)^3+3+k$.
$k=-3$

## Describe the transformations that map $y=3\ln(7-x)+2$ onto $y=6\ln(x+2)-1$.

$y'=6\ln(x'+2)-1$
$\dfrac{y'+1}{6}=\ln(x'+2)$

$y=3\ln(7-x)+2$
$\dfrac{y-2}{3}=\ln(7-x)$
$\to$
$\dfrac{y'+1}{6}=\ln(x'+2)$

$\dfrac{y-2}{3}=\dfrac{y'+1}{6}$
$2y-4=y'+1$
$y'=2y-5$

$\ln(7-x)=\ln(x'+2)$
$7-x=x'+2$
$x'=-x+5$

- Dilate 2 from x axis.
- Reflect in y axis.
- Translate 5 right and 5 down.

## What is $y=6x^2$ after dilation 2 in y axis?

$x,y\to x'=2x,y'=y$
$x=\dfrac{x'}{2}$
$y=6x^2$
$\to$
$y=6(\dfrac{x}{2})^2$
$y=\dfrac{3x^2}{2}$

## The function $f(x)$ is transformed by $T(x,y)$ into $-a^2f(bx-c^2)-d$. Describe the transformations.

We can see that $x\to x'=bx-c^2$.
And $f\to f'=-a^2f-d$.

## The tangent at the point $(−1,0)$ on the curve $y=f(x)$ has the equation $y=3x+c$. Find the equation of the tangent at the point $(3,1)$ to the curve $y=−2\dfrac{1}{2}f(−x+2)+1$.

Let the transformed function be $g(x)=−2\dfrac{1}{2}f(−x+2)+1$

$g'(x)=-\dfrac{1}{2}\cdot f'(-x+2)\cdot -1$
$g'(x)=\dfrac{1}{2}f'(-x+2)$

$g'(3)=\dfrac{1}{2}f'(-3+2)$
$g'(3)=\dfrac{1}{2}f'(-1)$

$f'(-1)=3$

$g'(3)=\dfrac{3}{2}$

Now find the line. Use the point $(3,1)$ and $m=\dfrac{3}{2}$

$y-y_1=m(x-x_1)$

$y-1=\dfrac{3}{2}(x-3)$
$y=\dfrac{3}{2}x-\dfrac{9}{2}+1$
$y=\dfrac{3}{2}x-\dfrac{7}{2}$

## What is the transformation $T$ that maps $y=\tan(5x-2)+4$ onto $y=2\tan(3x)$?

$y'=2\tan(3x')$
$\dfrac{y'}{2}=\tan(3x')$

$y=\tan(5x-2)+4$
$y-4=\tan(5x-2)$
$\to$
$\dfrac{y'}{2}=\tan(3x')$

$\dfrac{y'}{2}=y-4$
$y'=2y-8$
$5x-2=3x'$
$x'=\dfrac{5}{3}x-\dfrac{2}{3}$

$T(x,y)=(\dfrac{5}{3}x-\dfrac{2}{3},2y-8)$

## Describe the transformations that map $y=6\tan(\dfrac{1}{3}x-\dfrac{\pi}{6})+5$ onto $y=2\tan(3x-\dfrac{\pi}{3})+7$.

$y'=2\tan(3x'-\dfrac{\pi}{3})+7$
$\dfrac{y'-7}{2}=\tan(3x'-\dfrac{\pi}{3})$

$y=6\tan(\dfrac{1}{3}x-\dfrac{\pi}{6})+5$
$\dfrac{y-5}{6}=\tan(\dfrac{1}{3}x-\dfrac{\pi}{6})$
$\to$
$\dfrac{y'-7}{2}=\tan(3x'-\dfrac{\pi}{3})$

$\dfrac{y'-7}{2}=\dfrac{y-5}{6}$
$3y'-21=y-5$
$y'=\dfrac{y}{3}+\dfrac{16}{3}$


$\tan(\dfrac{1}{3}x-\dfrac{\pi}{6})=\tan(3x'-\dfrac{\pi}{3})$

$\dfrac{1}{3}x-\dfrac{\pi}{6}=3x'-\dfrac{\pi}{3}$
$3x'=\dfrac{1}{3}x+\dfrac{\pi}{6}$
$x'=\dfrac{1}{9}x+\dfrac{\pi}{18}$

- Dilate $\dfrac{1}{9}$ from y axis.
- Dilate $\dfrac{1}{3}$ from x axis.
- Translate $\dfrac{\pi}{18}$ right and $\dfrac{16}{3}$ up.

## What is $y=(x+4)^2+2$ after dilation 3 from x axis?

$x,y\to x'=x,y'=3y$
$y=\dfrac{y'}{3}$

$y=(x+4)^2+2$
$\to$
$\dfrac{y}{3}=(x+4)^2+2$
$y=3(x+4)^2+6$

## Consider the transformation $T(x,y)=(3+x,4-y)$. Find the inverse transformation $T^{-1}$.

$x'=3+x$
$y'=4-y$

$x=x-3$
$y=4-y'$

Therefore.
$T^{-1}(x,y)=(x-3,4-y')$

## Consider the transformation $T(x,y)=(\dfrac{3x+4}{3},\dfrac{5y-4}{4})$. Find the inverse transformation $T^{-1}$.

$x'=\dfrac{3x+4}{3}$
$y'=\dfrac{5y-4}{4}$

$x=\dfrac{3x-4}{3}$
$y=\dfrac{4y+4}{5}$

Therefore.

$T^{-1}(x,y)=(\dfrac{3x-4}{3},\dfrac{4y+4}{5})$

## Let $f(x)=x^2-4$ and $g(x)=4(x−1)^2−4$, let the graph of g be a transformation of the graph of f where the transformations have been applied in the following order: Dilation $n$ from the x axis, translation 1 right and $m$ up. $n$ and $m$ are positive real numbers. What is $m-n$?

Let f be y and g be y'

$y'=4(x'-1)^2-4$

$(x,y)\to x'=x+1,y'=ny+m$
$x=x'-1$
$y=\dfrac{y'-m}{n}$

$y=x^2-4$

$\dfrac{y'-m}{n}=(x'-1)^2-4$
$y'=n(x'-1)^2-4n+m$
$y'=4(x'-1)^2-4$

$4(x'-1)^2-4=n(x'-1)^2-4n+m$
$4(x-1)^2-4=n(x^2-2x+1)-4n+m$
$4(x-1)^2-4=nx^2-2nx+n-4n+m$
$4x^2-8x=nx^2-2nx-3n+m$

$4=n$
$-8=-2n$
$-3n+m=0$

$-12+m=0$
$m=12$
$m-n=8$

## Given that $g(x)=2x−2$ and $f(x)=x^2+2x+3$, for what dilation factor(s) from the x-axis does the graph of g(x) need to undergo if g(x) and f(x) intersect exactly once?

Let dilation factor needed be d
Let y be g(x) and dilated g(x) be y'

$y=2x-2$
$(x,y)\to x'=x,y'=dy$
$\dfrac{y'}{d}=2x'-2$

$y'=2dx'-2d$

Intersection.

$x^2+2x+3=2dx-2d$
$x^2+(2-2d)x+3+2d=0$

There is one solution to this equation. Discriminant be zero.
$\Delta=0$
$\Delta=(2-2d)^2-4(1)(3+2d)$
$0=4-8d+4d^2-12-8d$
$0=4d^2-16d-8$
$0=d^2-4d-2$

Use quadratic formula.

$d=\dfrac{4\pm\sqrt{16-4(-2)}}{2}$
$d=2\pm\sqrt{6}$

The word dilation implies the dilation factor is positive, therefore.

$d=2+\sqrt{6}$
