---
title: 
description: 
aliases: []
tags: []
created: 2025-05-14T16:13:00
modified: 2025-05-21T16:40:05
permalink:
---

## Find derivative of $f(x)=\ln(2x-7)$.

$f'(x)=\dfrac{1}{2x-7}\cdot (2)=\dfrac{2}{2x-7}$

## For $f(x)=x^2-2$, use Newton's method to approximate $x_1$ starting with $x_0=-1$.

$x_1=x_0-\dfrac{f(x_0)}{f'(x_0)}$

$x_1=-1-\dfrac{(-1)^2-2}{2(-1)}$
$x_1=\dfrac{-3}{2}$

## Find $f''(-2)$ for $f(x)=e^{3x}+5x^2-\dfrac{3}{x}$.

$f'(x)=3e^{3x}+10x+(-3)(-1)(x)^{-2}$
$f'(x)=3e^{3x}+10x+3x^{-2}$
$f''(x)=9e^{3x}+10-6x^{-3}$

$f''(2)=9e^6+10+\dfrac{-6}{(-2)^3}$
$f''(2)=9e^6+\dfrac{40}{4}-\dfrac{3}{4}$
$f''(2)=9e^6+\dfrac{37}{4}$

## For $f(x)=\sqrt{-x}$, find angle $\theta$ from the positive x axis to the tangent of f when $x=\dfrac{-3}{4}$.

$f'(x)=\dfrac{1}{2}(-x)^{\dfrac{-1}{2}}(-1)$
$f'(x)=\dfrac{1}{-2\sqrt{-x}}$

$\tan(\theta)=f'(\dfrac{-3}{4})=\dfrac{1}{-2(\dfrac{\sqrt{3}}{2})}$
$\tan(\theta)=\dfrac{1}{\dfrac{-\sqrt{3}}{1}}=\dfrac{-1}{\sqrt{3}}$

$\theta=\dfrac{5\pi}{6}$

## Let $f(x)=-\ln(x+3)$. A tangent to the graph has y-intercept at $(0,c)$. What is the maximum value of c?

$f'(x)=\dfrac{-1}{x+3}$

## Find the coordinate of the point of inflection of $f(x)=-\dfrac{x^3}{2}-\dfrac{x^2}{4}-x$.

$f'(x)=\dfrac{-3x^2}{2}+\dfrac{-x}{2}-1$
$f''(x)=-3x-\dfrac{1}{2}=0$
$x=\dfrac{-1}{6}$ is a possible POI. Testing concavity before and after.
$f''(0)<0$
$f''(\dfrac{-1}{3})>0$

Concavity changes, hence is POI at $x=\dfrac{-1}{6}$

$f(\dfrac{-1}{6})=\dfrac{35}{216}$

## Find the equation of the tangent to the curve of $f(x)=(2x+3)^{\dfrac{3}{5}}+3$ at $x=\dfrac{-3}{2}$.

$y-y_1=m(x-x_1)$

$m=f'(\dfrac{-3}{2})$

$f'(x)=\dfrac{3}{5}(2x+3)^{\dfrac{-2}{5}}(2)$
$f'(x)=\dfrac{6}{5}(2x+3)^{\dfrac{-2}{5}}$
$f'(\dfrac{-3}{2})=0$

A point is $(\dfrac{-3}{2},3)$

$y-3=0$
$y=3$

## Differentiate $f(x)=\dfrac{4e^{2x}-2e^x+1}{2e^{2x}}$.

$f'(x)=\dfrac{(8e^{2x})(-2e^x)(2e^{2x})-(4e^{2x}-2e^x+1)(4e^{2x})}{4e^{4x}}$

## Differentiate $f(x)=e^{2x}+e^4+e^{-2x}$.

$f'(x)=2e^{2x}-2e^{2x}$

## Differentiate $f(x)=3\ln(4x)+x$.

$f'(x)=3(\dfrac{4}{4x})+1$
$f'(x)=\dfrac{3}{x}+1$

## Find $f''(x)$ for $f(x)=36xe^{-0.5x}$.

$f(x)=(36x)(e^{-0.5x})$
$f'(x)=(36)(e^{-0.5x})+(36x)(-0.5e^{-0.5x})$
$f'(x)=36e^{-0.5x}-18xe^{-0.5x}$
$f''(x)=-18e^{-0.5x}+(-18)(e^{-0.5x})+(-18x)(-0.5e^{-0.5x})$
$f''(x)=(9x-36)e^{-0.5x}$

## What is the equation of the tangent to the graph $y=\sqrt{e^x}-2x$ at the point $(0,1)$?

$\dfrac{dy}{dx}=\dfrac{1}{2}(e^x)^\dfrac{-1}{2}(e^x)-2$
$\dfrac{dy}{dx}=\dfrac{1}{2\sqrt{e^x}}(e^x)-2$
