---
title: 
description: 
aliases: []
tags: []
created: 2024-12-04T21:50:47
modified: 2025-02-09T15:53:45
permalink:
---

worked example: Differentiate $f(x)=\dfrac{2x}{x+1}$

$f'(x)=\dfrac{(2)(x+1)-(2x)(1)}{(x+1)^2}$

$f'(x)=\dfrac{2x+2-2x}{(x+1)^2}$

$f'(x)=\dfrac{2}{(x+1)^2}$



worked example: Differentiate $f(x)=\dfrac{x^2}{3x-1}$

$f'(x)=\dfrac{(2x)(3x-1)-(x^2)(3)}{(3x-1)^2}$

$f'(x)=\dfrac{6x^2-2x-3x^2}{(3x-1)^2}$

$f'(x)=\dfrac{3x^2-2x}{(3x-1)^2}$

worked example: Differentiate $f(x)=\dfrac{4e^{2x}-2e^x+1}{2e^{2x}}$

$f'(x)=\dfrac{(8e^{2x}-2e^x)(2e^{2x})-(4e^{2x}-2e^x)(4e^{2x})}{(2e^{2x})^2}$

$f'(x)=\dfrac{16e^{4x}-4e^{3x}-16e^{4x}+8e^{3x}}{2e^{4x}}$

$f'(x)=\dfrac{2e^{3x}}{e^{4x}}$

worked example: Differentiate $f(x)=\dfrac{(x-1)^2}{x^2+1}$


$f'(x)=\dfrac{(2x-2)(x^2+1)-(x-1)^2\cdot (2x)}{(x^2+1)^2}$
