---
title: 
description: 
aliases: []
tags: []
created: 2025-03-06T08:49:34
modified: 2025-03-06T08:59:19
permalink:
---

## Simplify $\dfrac{1-i}{1+i}$.

$=\dfrac{1-i}{1+i}\cdot \dfrac{1-i}{1-i}$

$=\dfrac{1-2i-1}{1^2-i^2}$

$=\dfrac{-2i}{1+1}$

$=\dfrac{-2i}{2}$

$=-i$

## Simplify $\dfrac{(1-i)^9}{(1+i)^8}$

$$
\begin{aligned} \frac{(1-i)^{9}}{(1+i)^{8}} &= \frac{(1-i)^{8}(1-i)}{(1+i)^{8}} \\ &= \left[\frac{(1-i)}{(1+i)}\right]^{8} (1-i) \\ &= \left[\frac{(1-i)(1-i)}{(1+i)(1-i)}\right]^{8} (1-i) \\ &= \left[\frac{1 - 2i + i^2}{1 - i^2}\right]^{8} (1-i) \\ &= \left[\frac{1 - 2i - 1}{1 - (-1)}\right]^{8} (1-i) \\ &= \left[\frac{-2i}{2}\right]^{8} (1-i) \\ &= (-i)^{8} (1-i) \\ &= ( (-1)i )^{8} (1-i) \\ &= ( (-1)^{8} i^{8} ) (1-i) \\ &= (1 \cdot (i^{4})^{2}) (1-i)\\ &= (1 \cdot (1)^{2}) (1-i)\\ &= 1 \cdot (1-i) \\ &= 1-i \end{aligned}
$$
