---
title: 
description: 
aliases: []
tags: []
created: 2025-01-31T11:16:03
modified: 2025-02-09T15:53:44
permalink:
---

1. simplify the following
	1. $(3x^4)^4$
	$=81x^{16}$
	1. $13x^\dfrac{2}{3}\cdot 5x^\dfrac{1}{5}$
	$=65x^{\dfrac{13}{15}}$
	
	1. $(x^5)^\dfrac{2}{7}\cdot x^\dfrac{-1}{9}$
	$=x^{\dfrac{10}{7}}\cdot x^{\dfrac{-1}{9}}$
	$=x^{\dfrac{83}{63}}$


2. simplify the following
	1. $\dfrac{3}{x-4}+\dfrac{5x}{4-x}$
	$=\dfrac{3-5x}{x-4}$
	1. $\dfrac{7}{x+1}-\dfrac{8x}{5x-2}$
	$=\dfrac{35x-14-8x^2-8x}{(x+1)(5x-2)}$
	$=\dfrac{-8x^2+27x-14}{(x+1)(5-2)}$
	1. $\dfrac{3x+2}{2x^2+5x-3}-\dfrac{4x-3}{6x^2+3x-3}$
	$=\dfrac{3x+2}{(2x-1)(x+3)}-\dfrac{4x-3}{(2x-1)(3x+3)}$
	$=\dfrac{(3x+2)(3x+3)-(4x-3)(x+3)}{(2x-1)(x+3)(3x+3)}$
	$=\dfrac{9x^2+15x+6-(4x^2+8x-9)}{(2x-1)(x+3)(3x+3)}$
	$=\dfrac{5x^2+7x+15}{(2x-1)(x+3)(3x+3)}$
3. solve for x
	1. $\dfrac{4x}{3}+\dfrac{x}{6}=7$
	$9x=42$
	$x=\dfrac{14}{3}$
	1. $\dfrac{3x-1}{4}-\dfrac{5-2x}{3}=1$
	$\dfrac{9x-3-20+8x}{12}=1$
	$17x-23=12$
	$x=\dfrac{35}{17}$
	1. $\dfrac{4}{7x}-\dfrac{3}{2x}=\dfrac{3}{4}$
	$\dfrac{8-21}{14x}=\dfrac{3}{4}$
	$-52=42x$
	$x=\dfrac{-52}{42}$
	$x=\dfrac{-26}{21}$
	
4. express as a single fraction
	1. $(x+2)^\dfrac{1}{4}+(x+2)^\dfrac{-3}{4}$
	$=(x+2)^{\dfrac{1}{4}}+\dfrac{1}{(x+2)^{\dfrac{3}{4}}}$
	$=\dfrac{x+3}{(x+2)^{\dfrac{3}{4}}}$
	
	1. $(3-2x)^\dfrac{1}{2}-(3-2x)^\dfrac{-3}{2}$
	$=(3-2x)^\dfrac{1}{2}-\dfrac{1}{(3-2x)^{\dfrac{3}{2}}}$
	$=\dfrac{9-4x^2-12x-1}{(3-2x)^{\dfrac{3}{2}}}$
	


5. solve for x
	1. $3a-x=\dfrac{bx}{c}+3$
	$\dfrac{bx}{c}+x=3a-3$
	$\dfrac{x(b+c)}{c}=3a-3$
	$x=\dfrac{3ac-3c}{b+c}$
	1. $u=\dfrac{-2x-3}{bx}$
	$ubx=-2x-3$
	$x(ub+2)=-3$
	$x=\dfrac{-3}{ub+2}$
	1. $\dfrac{a}{x}+\dfrac{b}{2}=\dfrac{5}{a}$
	$\dfrac{2a+bx}{2x}=\dfrac{5}{a}$
	$2a^2+abx=10x$
	$x(10-ab)=2a^2$
	$x=\dfrac{2a^2}{10-ab}$


6. solve for x and y
	1. $4ax+2by=5$ and $3ax+by=-8$
	$6ax+2by=-16$
	$x=\dfrac{-21}{2a}$
	$by=-8+\dfrac{63}{2}=\dfrac{47}{2}$
	$y=\dfrac{47}{2b}$
	
	2. $ax-2by=1$ and $x+y=7$
	$ax+ay=7a$
	$-2by-ay=1-7a$
	$ax-2by=1$
	$y=7-x$
	$ax-2b(7-x)=1$
	$ax-14b+2bx=1$
	$(a+2b)x=14b+1$
	$x=\dfrac{14b+1}{a+2b}$
	$y=\dfrac{7a-1}{a+2b}$

7. expand the following
	1. $(x+2y)^3$
	$=x^3+3x^2(2y)+3x(2y)^2+y^3$
	$=x^3+6x^2y+12xy^2+y^3$
	1. $(3x-y)^3$
	$=(3x)^3-3(3x)^2(y)+3(3x)(y)^2-y^3$
	$=27x^3-27x^2y+9xy^2-y^3$
	1. $(\dfrac{2}{x}+3)^4$
	$=(\dfrac{2}{x})^4+4(\dfrac{2}{x})^3(3)+6(\dfrac{2}{x})^2(3)^2+4(\dfrac{2}{x})(3)^3+3^4$
	$=\dfrac{8}{x^4}+\dfrac{96}{x^3}+\dfrac{108}{x^2}+\dfrac{216}{x}+81$
	
8. if $2(x+2)^2+3x+4=ax^2+bx+c$, find the values of a, b, and c
	$=2(x^2+4x+4)+3x+4$
	$=2x^2+11x+12$
	a=2
	b=11
	c=12
9. express $(x+1)^3$ in the form $(x+2)^3+a(x+2)^2+b(x+2)+c$
	let u=x+2
	$(x+1)^3=u^3+au^2+bu+c$
	$(u-1)^3=u^3+au^2+bu+c$
	$u^3-3u^2+3x-1=u^3+au^2+bu+c$
	a=-3
	b=3
	c=-1
