---
title: 
description: 
aliases: []
tags: []
created: 2025-01-30T13:13:11
modified: 2025-02-09T15:53:44
permalink:
---


1. simplify the following
	1. $(x^5)^7$
	$=x^{35}$
	1. $y^9\cdot y^4$
	$=y^{13}$
	1. $(3a^7)^4$
	$=81a^{28}$
	1. $7x^{11}\cdot 8x^{15}$
	$=56x^{26}$
	1. $(25x^{\frac{1}{3}})^{\dfrac{3}{2}}$
	$=125x^{\dfrac{1}{2}}$
	1. $14a^\dfrac{3}{5}\cdot 12a^{-\dfrac{1}{9}}$
	$=168a^{\dfrac{22}{45}}$

2. simplify the following
	1. $\dfrac{2x}{3}+\dfrac{3x}{2}$
	$=\dfrac{4x+9x}{6}$
	$=\dfrac{13x}{6}$
	2. $\dfrac{3a}{2}-\dfrac{a}{4}$
	$=\dfrac{5a}{4}$
	3. $\dfrac{3x}{4}-\dfrac{y}{6}-\dfrac{x}{3}$
	$=\dfrac{9x-2y-4x}{12}$
	$=\dfrac{5x-2y}{12}$
	4. $\dfrac{3}{x}+\dfrac{2}{y}$
	$=\dfrac{3y+2x}{xy}$
	5. $\dfrac{3}{x-2}+\dfrac{2}{x+1}$
	$=\dfrac{3(x+1)+2(x-2)}{(x+1)(x-2)}$
	$=\dfrac{3x+3+2x-4}{(x+1)(x-2)}$
	$=\dfrac{5x-1}{(x+1)(x-2)}$
	6. $\dfrac{3}{x-1}+\dfrac{2}{(x-1)(x+4)}$
	$=\dfrac{3(x+4)+2}{(x-1)(x+4)}$
	$=\dfrac{3x+14}{(x-1)(x+4)}$
	7. $\dfrac{3}{x-2}-\dfrac{2}{x+2}+\dfrac{4}{x^2-4}$
	$=\dfrac{3(x+2)-2(x-2)}{(x-2)(x+2)}+\dfrac{4}{(x-2)(x+2)}$
	$=\dfrac{3x+6-2x+4+4}{(x-2)(x+2)}$
	$=\dfrac{x+14}{(x-2)(x+2)}$
	8. $\dfrac{5}{x+2}+\dfrac{3}{x^2+5x+6}-\dfrac{2-x}{x+3}$
	$=\dfrac{5(x+3)+3-(x+2)(2-x)}{(x+3)(x+2)}$
	$=\dfrac{5x+18-(-x^2+4)}{(x+3)(x+2)}$
	$=\dfrac{5x+18+x^2-4}{(x+3)(x+2)}$
	$=\dfrac{x^2+5x+14}{(x+3)(x+2)}$
	9. $\dfrac{x-y}{2}-\dfrac{1}{x-y}$
	$=\dfrac{(x-y)^2-2}{2(x-y)}$
	$=\dfrac{x^2-2xy-y^2-2}{2x-2y}$
	10. $\dfrac{3}{x-1}-\dfrac{4x}{1-x}$
	$=\dfrac{3+4x}{x-1}$
	11. $\dfrac{2}{x^2+3x+2}+\dfrac{3}{x^2+7x+10}$
	$=\dfrac{2}{(x+1)(x+2)}+\dfrac{3}{(x+2)(x+5)}$
	$=\dfrac{2(x+5)+3(x+1)}{(x+1)(x+2)(x+5)}$
	$=\dfrac{5x+13}{(x+1)(x+2)(x+5)}$
	12. $\dfrac{x}{2x^2+x-3}-\dfrac{5}{2x^2-5x-12}$
	$=\dfrac{x}{(2x+3)(x-1)}-\dfrac{5}{(2x+3)(x-4)}$
	$=\dfrac{x(x-4)-5(x-1)}{(2x+3)(x-1)(x-4)}$
	$=\dfrac{x^2-9x+5}{(2x+3)(x-1)(x-4)}$
	13. $\dfrac{5}{x+3}+\dfrac{4x}{3x-2}+\dfrac{2}{2-3x}$
	$=\dfrac{5}{x+3}+\dfrac{4x-2}{3x-2}$
	$=\dfrac{15x-10+(x+3)(4x-2)}{(x+3)(3x-2)}$
	$=\dfrac{15x-10+4x^2-2x+12x-6}{(x+3)(3x-2)}$
	$=\dfrac{4x^2+25x-16}{(x+3)(3x-2)}$
	1. $\dfrac{5-x}{4-x}+\dfrac{3x+1}{x+4}-\dfrac{2}{x-4}$
	$=\dfrac{x-7}{x-4}+\dfrac{3x+1}{x+4}$
	$=\dfrac{x^2-3x-28+3x^2-11x-4}{(x-4)(x+4)}$
	$=\dfrac{4x^2-14x-32}{(x-4)(x+4)}$
	1. $\dfrac{x-3}{3x^2+5x-2}+\dfrac{4-2x}{-3x^2+16x-5}$
	$=\dfrac{x-3}{3x^2+5x-2}+\dfrac{2x-4}{3x^2-16x+5}$
	$=\dfrac{x-3}{(3x-1)(x+3)}+\dfrac{2x-4}{(3x-1)(x-5)}$
	$=\dfrac{x^2-8x+15+2x^2-x-12}{(3x-1)(x+3)(x-5)}$
	$=\dfrac{3x^2-9x+3}{(3x-1)(x+3)(x-5)}$

3. simplify the following
	1. $\dfrac{x^2}{2x}\cdot \dfrac{4y^3}{x}$
	$=2y^3$
	1. $\dfrac{3x^2}{4y}\cdot \dfrac{y^2}{6x}$
	$=\dfrac{xy}{8}$
	1. $\dfrac{x^2}{2y}\div\dfrac{3xy}{6}$
	$=\dfrac{x}{y^2}$
	1. $\dfrac{4-x}{3a}\cdot \dfrac{a^2}{4-x}$
	$=\dfrac{a}{3}$
	1. $\dfrac{(x-1)^2}{x^2+3x-4}$
	$=\dfrac{x-1}{x+4}$
	1. $\dfrac{x^2-x-6}{x-3}$
	$=x+2$
	1. $\dfrac{x-2}{x}\div \dfrac{x^2-4}{2x^2}$
	$=\dfrac{2x-4}{x-4}$
	1. $\dfrac{x+2}{x^2-3x}\div \dfrac{4x+8}{x^2-4x+3}$
	$=\dfrac{x+2}{x(x-3)}\cdot \dfrac{(x-3)(x-1)}{4(x+2)}$
	$=\dfrac{x-1}{x}$
	1. $\dfrac{2x}{x-1}\div \dfrac{4x^2}{x^2-1}$
	$=\dfrac{2x}{x-1}\cdot \dfrac{(x+1)(x-1)}{4x^2}$
	$=\dfrac{x+1}{2}$
	1. $\dfrac{x^2-9}{x+2}\cdot \dfrac{3x+6}{x-3}\div \dfrac{9}{x}$
	$=\dfrac{(x+3)(x-3)}{x+2}\cdot \dfrac{3(x+2)}{x-3}\cdot \dfrac{x}{9}$
	$=\dfrac{x^2+3x}{3}$
	1. $\dfrac{3x}{9x-6}\div \dfrac{6x^2}{x-2}\cdot \dfrac{2}{x+5}$
	$=\dfrac{3x}{9x-6}\cdot \dfrac{x-2}{6x^2}\cdot \dfrac{2}{x+5}$
	$=\dfrac{x-2}{x(9x^2+39x-30)}$
	1. $\dfrac{2x^2+3x-5}{x^2+x}\div \dfrac{2x^2+7x+5}{x^2+2x+1}$
	$=\dfrac{(2x+5)(x-1)}{x(x+1)}\cdot \dfrac{(x+1)(x+1)}{(2x+5)(x+1)}$
	$=\dfrac{x-1}{x}$
	1. $\dfrac{x+2}{3x+5}\cdot \dfrac{6x+10}{x^2-4}\div \dfrac{8x}{4-2x}$
	$=\dfrac{x+2}{3x+5}\cdot \dfrac{2(3x+5)}{(x+2)(x-2)}\cdot \dfrac{4-2x}{8x}$
	$=\dfrac{4-2x}{4x(x-2)}$
	1. $\dfrac{x^2-9}{4-x^2}\div \dfrac{3+2x-x^2}{x^2+x-6}$
	$=\dfrac{(x+3)(x-3)}{(2-x)(2+x)}\cdot \dfrac{(x+3)(x-2)}{(x+3)(-x-1)}$
	$=\dfrac{(x+3)(x-3)(x-2)}{(2-x)(x+2)(-x-1)}$
	1. $\dfrac{2x^2+x-3}{x^2+2x}\div \dfrac{x^2-4x+3}{x^2}\div \dfrac{2x^2+3x}{x^2-x-6}$
	$=\dfrac{(2x+3)(x-1)}{x(x+2)}\cdot \dfrac{x^2}{(x-3)(x-1)}\cdot \dfrac{(x-3)(x+2)}{x(2x+3)}$
	$=1$

4. solve the following equations
	1. $\dfrac{x}{3}-2=-7$
	$\dfrac{x}{3}=-5$
	$x=-15$
	2. $\dfrac{5x-2}{4}+\dfrac{1}{2}=-2$
	$\dfrac{5x-2}{4}=-\dfrac{5}{2}$
	$5x-2=-10$
	$5x=-8$
	$x=\dfrac{-8}{5}$
	3. $\dfrac{5x}{4}-1=\dfrac{3}{7}$
	$5x=\dfrac{40}{7}$
	$x=\dfrac{8}{7}$
	4. $\dfrac{2x-1}{3}=\dfrac{5x+1}{7}$
	$14x-7=15x+3$
	$x=-10$
	5. $\dfrac{2x+1}{3}+7=11$
	$2x+1=12$
	$x=\dfrac{11}{2}$
	6. $\dfrac{2x+1}{3}+7=\dfrac{3x-1}{4}$
	$4(2x+1+\dfrac{7}{3})=9x-3$
	$8x+4+\dfrac{28}{3}=9x-3$
	$x=7+\dfrac{28}{3}$
	$x=\dfrac{49}{3}$
	7. $\dfrac{x+2}{5}+\dfrac{x-1}{2}=\dfrac{x+1}{3}$
	$\dfrac{2x+4+5x-5}{10}=\dfrac{x+1}{3}$
	$6x+12+15x-15=10x+10$
	$11x=13$
	$x=\dfrac{13}{11}$
	8. $x+5=\dfrac{14}{x}$
	$x^2+5x-14=0$
	$(x+7)(x-2)=0$
	$x=2\lor x=-7$
	9. $\dfrac{x+1}{3}=\dfrac{10}{x}$
	$x^2+x=30$
	$x^2+x-30=0$
	$(x+6)(x-5)=0$
	$x=-6\lor x=5$
	10. $\dfrac{1}{x+1}=\dfrac{5x-6}{6x}$
	$6x=5x^2-6x+5x-6$
	$0=5x^2-7x-6$
	$0=(5x-3)(x+2)$
	$x=\dfrac{3}{5}\lor x=-2$
	11. $\dfrac{2x}{3}+\dfrac{x-1}{15}=\dfrac{2}{3}+\dfrac{22}{x}$
	$\dfrac{11x-1}{15}=\dfrac{2x+66}{3x}$
	$33x^2-3x=30x+990$
	$33x^2-33x-990=0$
	$x^2-x-30=0$
	$(x+5)(x-6)=0$
	$x=-5\lor x=6$
	1. $\dfrac{x+1}{7}+\dfrac{8}{x-2}=3$
	$\dfrac{x^2-x-2+56}{7x-14}=3$
	$x^2-x-2+56=21x-42$
	$x^2-22x+96=0$
	$(x-6)(x-16)=0$
	$x=6\lor x=16$

5. express the following as a single fraction
	
	1. $\sqrt{1-x}+\dfrac{2}{\sqrt{1-x}}$
	$=\sqrt{1-x}+\dfrac{2\sqrt{1-x}}{1-x}$
	$=\dfrac{3\sqrt{1-x}}{1-x}$
	1. $\dfrac{2}{\sqrt{x-4}}+\dfrac{2\sqrt{x-4}}{3}$
	$=\dfrac{6}{3\sqrt{x-4}}+\dfrac{2(x-4)}{3\sqrt{x-4}}$
	$=\dfrac{2x-2}{3\sqrt{x-4}}$
	1. $\dfrac{3}{\sqrt{x+4}}+\dfrac{2}{\sqrt{x+4}}$
	$=\dfrac{5}{\sqrt{x+4}}$
	1. $\dfrac{3}{\sqrt{x-5}}+\sqrt{x-5}$
	$=\dfrac{3}{\sqrt{x-5}}+\dfrac{x-5}{\sqrt{x-5}}$
	$=\dfrac{x-2}{\sqrt{x-5}}$
	1. $\dfrac{3x^3}{\sqrt{2x-1}}-3x^2\sqrt{2x-1}$
	$=\dfrac{3x^3}{\sqrt{2x-1}}-\dfrac{3x^2(2x-1)}{\sqrt{2x-1}}$
	$=\dfrac{3x^3-6x^3+3x^2}{\sqrt{2x-1}}$
	$=\dfrac{-3x^3+3x^2}{\sqrt{2x-1}}$
	1. $\dfrac{4x^4}{3\sqrt{x+3}}+3x^2\sqrt{x+3}$
	$=\dfrac{4x^4}{3\sqrt{x+3}}+\dfrac{9x^2(x+3)}{3\sqrt{x+3}}$
	$=\dfrac{4x^4+9x^3+27x^2}{3\sqrt{x+3}}$
	

6. express the following as a single fraction
	1. $(6x-3)^\dfrac{1}{3}-(6x-3)^{-\dfrac{2}{3}}$
	$=(6x-3)^\dfrac{1}{3}-\dfrac{1}{(6x-3)^\frac{2}{3}}$
	$=\dfrac{6x-3}{(6x-3)^\frac{2}{3}}-\dfrac{1}{(6x-3)^\frac{2}{3}}$
	$=\dfrac{6x-4}{(6x-3)^\frac{2}{3}}$
	2. $(2x+3)^\dfrac{1}{4}-2x(2x+3)^{-\dfrac{3}{4}}$
	$=(2x+3)^\frac{1}{4}-\dfrac{2x}{(2x+3)^\frac{3}{4}}$
	$=\dfrac{2x+3-2x}{(2x+3)^\frac{3}{4}}$
	$=\dfrac{3}{(2x+3)^\frac{3}{4}}$
	3. $(3-x)^{-\dfrac{2}{5}}-5x(3-x)^\dfrac{3}{5}$
	$=\dfrac{1}{(3-x)^\frac{2}{5}}-\dfrac{5x(3-x)}{(3-x)^\frac{2}{5}}$
	$=\dfrac{5x^2-15x+1}{(3-x)^\frac{2}{5}}$
