---
title: 
description: 
aliases: []
tags: []
created: 2025-01-30T13:13:11
modified: 2025-02-09T15:53:44
permalink:
---

1. $(a+b)^4$
	$=a^4+4a^3b+6a^2b^2+4ab^3+b^4$

2. $(x+y)^6$
	$=a^6+6x^5y+15x^4y^2+20x^3y^3+15x^2y^4+6xy^5+y^6$

3. $(a-b)^4$
	$=a^4-4a^3b+6a^2b^2-4ab^3+b^4$

4. $(x-y)^5$
	$=x^5+5x^4(-y)+10x^3(-y)^2+10x^3(-y)^3+5x(-y)^4+(-y)^5$
	$=x^5-5x^4y+10x^3y^2-10x^3y^3+5xy^4-y^5$

5. $(a+3b)^3$
	$=a^3+3a^2(2b)+3a(3b)^2+(3b)^3$
	$=a^3+6a^2b+9ab^2+27b^3$

6. $(2x-y)^4$
	$=(2x)^4+4(2x)^3(-y)+6(2x)^2(-y)^2+4(2x)(-y)^3+(-y)^4$
	$=16x^4-32x^3y+24x^2y^2-8xy^3+y^4$

7. $(3a-2b)^3$
	$=(3a)^3+3(3a)^2(-2b)+3(3a)(-2b)^2+(-2b)^3$
	$=3a^3-54a^2b+36ab^2-8b^3$

8. $(\dfrac{1}{x}+x)^4$
	$=(\dfrac{1}{x})^4+4(\dfrac{1}{x})^3(x)+6(\dfrac{1}{x})^2(x)^2+4(\dfrac{1}{x})(x)^3+x^4$
	$=\dfrac{1}{x^4}+\dfrac{4}{x^2}+6+4x^2+x^4$

9. $(2^x+2)^4$
	$=(2^x)^4+4(2^x)^3(2)+6(2^x)^2(2)^2+4(2^x)(2)^3+2^4$
	$=2^{4x}+8(2^{3x})+24(2^{2x})+32(2^x)+16$

10. $(2x-\dfrac{1}{x})^3$
	$=(2x)^3+3(2x)^2(\dfrac{-1}{x})+3(2x)(\dfrac{-1}{x})^2+(\dfrac{-1}{x})^3$
	$=8x^3-12x+\dfrac{6}{x}-\dfrac{1}{x^3}$

11. $(3-3^x)^5$
	$=3^5+5(3)^4(-3^x)+10(3)^3(-3^x)^2+10(3)^2(-3^x)^3+5(3)(-3^x)^4+(-3^x)^5$
	$=243-405(3^x)+270(3^{2x})-90(3^{3x})+15(3^{4x})-3^{5x}$

12. $(\dfrac{2}{x}-x)^5$
	$=(\dfrac{2}{x})^5+5(\dfrac{2}{x})^4(-x)+10(\dfrac{2}{x})^3(-x)^2+10(\dfrac{2}{x})^2(-x)^3+5(\dfrac{2}{x})(-x)^4+(-x)^5$
	$=\dfrac{32}{x^5}+\dfrac{-80x}{x}+\dfrac{80x^2}{x}+\dfrac{-40x^3}{x}+\dfrac{10x^4}{x}-x^5$
	$=\dfrac{32}{x^5}-80+80x-40x^2+10x^3-x^5$

13. $(x+y)^5+(2x-y)^5$
	$=x^5+5x^4y+10x^3y^2+10x^2y^3+5xy^4+y^5+(2x)^5+5(2x)^4(-y)+10(2x)^3(-y)^2+10(2x)^2(-y)^3+5(2x)(-y)^4+(-y)^5)$
	$=33x^5-75x^4y+80x^3y^2-30x^2y^3+15xy^4$

14. $(x-y)^7+(x+y)^7$
	$=x^7-7x^6y+21x^5y^2-35x^4y^3+35x^3y^4-21x^2y^5+7xy^6-y^7+7x^6y+21x5y^2-35x^4y^3+35x^3y^4-21x^2y^5+7xy^6-y^7$
	$=2x^7+42x^5y^2+70x^3y^4+14xy^6$
