---
title: 
description: 
aliases: []
tags: []
created: 2025-01-30T13:13:11
modified: 2025-02-09T15:53:44
permalink:
---


1. Solve each of the following for $x$
	1. $ax+n=m$
		$ax=m-n$
		$x=\dfrac{m-n}{a}$
	1. $ax+b=bx$
		$ax-bx=-b$
		$x=\dfrac{-b}{a-b}$
		$x=\dfrac{b}{b-a}$
	1. $\dfrac{ax}{b}+c=0$
		$ax=-cb$
		$x=\dfrac{-cb}{a}$
	1. $px=qx+5$
		$x(p-q)=5$
		$x=\dfrac{5}{p-q}$
	1. $mx+n=nx-m$
		$mx-nx=-m-n$
		$x(m-n)=-m-n$
		$x=\dfrac{-m-n}{m-n}$
		$x=\dfrac{m+n}{n-m}$
	1. $\dfrac{1}{x+a}=\dfrac{b}{x}$
		$x=b(x+a)$
		$x=bx+ba$
		$x-bx=ba$
		$x=\dfrac{ba}{1-b}$
	1. $\dfrac{b}{x-a}=\dfrac{2b}{x+a}$
		$b(x+a)=2b(x-a)$
		$bx+ba=2bx-2ba$
		$2bx-bx=ba+2ba$
		$x=\dfrac{ba+2ba}{b}$
		$x=3a$
	1. $\dfrac{x}{m}+n=\dfrac{x}{n}+m$
		$xn+mn^2=xm+m^2n$
		$xn-xm=m^2n-mn^2$
		$x=\dfrac{m^2n-mn^2}{n-m}$
		$x=\dfrac{mn(m-n)}{n-m}$
		$x=\dfrac{-mn(n-m)}{n-m}$
		$x=-mn$
	1. $-b(ax+b)=a(bx-a)$
		$-bax-b^2=abx-a^2$
		$2abx=a^2-b^2$
		$x=\dfrac{a^2-b^2}{2ab}$
		
	1. $p^2(1-x)-2pqx=q^2(1+x)$
		$p^2-xp^2-2pqx=q^2+xq^2$
		$xq^2+2pqx+xp^2=p^2-q^2$
		$(x)(p+q)^2=(p+q)(p-q)$
		$x=\dfrac{p-q}{p+q}$
	1. $\dfrac{x}{a}-1=\dfrac{x}{b}+2$
		$bx-ab=ax+2ab$
		$bx-ax=3ab$
		$x=\dfrac{3ab}{b-a}$
	1. $\dfrac{x}{a-b}+\dfrac{2x}{a+b}=\dfrac{1}{a^2-b^2}$
		$xa+xb+2x(a-b)=\dfrac{(a+b)(a-b)}{(a+b)(a-b)}$
		$x(a+b+2a-2b)=1$
		$x=\dfrac{1}{3a-b}$
	1. $\dfrac{p-qx}{t}+p=\dfrac{qx-t}{p}$
		$p^2-pqx+p^2t=qtx-t^2$
		$qtx+pqx=p^2t+q^2+t^2$
		$x(qt+pq)=\dfrac{p^2t+q^2+t^2}{qt+pq}$
	1. $\dfrac{1}{x+a}+\dfrac{1}{x+2a}=\dfrac{2}{x+3a}$
		$(x+2a)(x+3a)+(x+a)(x+3a)=2(x+a)(x+2a)$
		$x^2+5ax+6a^2+x^2+4ax+3a^2=2x^2+6ax+4a^2$
		$5ax+6a^2+4ax+3a^2=6ax+4a^2$
		$3ax=-5a^2$
		$x=\dfrac{-5a}{3}$
2. Consider the simultaneous equations $ax+by=p$ and $bx-ay=q$
	1. Multiply the first equation by a and the second equation by b. Then eliminate y to solve for x.
		$a^2x+aby=ap$
		$b^2x-aby=bq$
		$x=\dfrac{ap+bq}{a^2+b^2}$
	1. Multiply the first equation by b and the second equation by -a. Then eliminate x to solve for y.
		$abx+b^2y=bp$
		$-abx+a^2y=aq$
		$y=\dfrac{bp+aq}{a^2+b^2}$
3. Consider the simultaneous equations $\dfrac{x}{a}+\dfrac{y}{b}=1$ and $\dfrac{x}{b}+\dfrac{y}{a}=1$
	1. Multiply the first equation by b and the second equation by -a. Then eliminate y to solve for x.
		$\dfrac{bx}{a}+y=1$
		$\dfrac{-ax}{b}-y=-a$
		$\dfrac{(b^2-a^2)x}{ab}=1-a$
		$x=\dfrac{ab-a^2b}{b^2-a^2}$
	1. Substitute solution for x into the first equation to solve for y.
		$\dfrac{ab-a^2b}{a(b^2-a^2)}+\dfrac{y}{b}=1$
		$\dfrac{b-ab}{b^2-a^2}+\dfrac{y}{b}=1$
		$y=\dfrac{ab^2-b^2}{b^2-a^2}$
1. Solve each of the following pairs of equations for $x$ and $y$
	1. $y=ax-b$ and $y=cx+a$
		$ax-b=cx+a$
		$x(a-c)=a+b$
		$x=\dfrac{a+b}{a-c}$
		$y=a(\dfrac{a+b}{a-c})-b$
		$y=\dfrac{a^2+ba-b(a-c)}{a-c}$
		$y=\dfrac{a^2+bc}{a-c}$
	1. $ax+y=c$ and $x+by=d$
		$x+b(c-ax)=d$
		$x+bc-abx=d$
		$x(1-ab)=d-bc$
		$x=\dfrac{d-bc}{1-ab}$
		$ax+y=c$
		$ax+aby=ad$
		$y-aby=c-ad$
		$y=\dfrac{c-ad}{1-ab}$
	1. $ax-by=a^2$ and $bx-ay=b^2$
		$a^2x-aby=a^3$
		$b^2x-aby=b^3$
		$a^2x-b^2x=a^3-b^3$
		$x=\dfrac{a^3-b^3}{a^2-b^2}$
		$x=\dfrac{(a-b)(a^2+ab+b^2)}{(a+b)(a-b)}$
		$x=\dfrac{a^2+ab+b^2}{a+b}$
		$abx-b^2y=a^2b$
		$abx-a^2y=ab^2$
		$-b^2y+a^2y=a^2b-ab^2$
		$y=\dfrac{a^2b-ab^2}{a^2-b^2}$
		$y=\dfrac{(ab)(a-b)}{(a+b)(a-b)}$
		$y=\dfrac{ab}{a+b}$
	1. $ax+by=t$ and $ax-by=s$
		$2by=t-s$
		$y=\dfrac{t-s}{2b}$
		$2ax=t+s$
		$x=\dfrac{t+s}{2a}$
	1. $y=abx+ac$ and $y=ax-bc$
		$by=abx-b^2c$
		$y-by=ac+b^2c$
		$y=\dfrac{ac+b^2c}{1-b}$
		$abx+ac=ax-bc$
		$x(ab-a)=-bc-ac$
		$x=\dfrac{ac+bc}{a-ab}$
	1. $ax+by=a^2+2ab-b^2$ and $bx+ay=a^2+b^2$
		$abx+b^2y=b(a^2+2ab-b^2)$
		$abx+a^2y=a(a^2+b^2)$
		$b^2y-a^2y=ba^2+2ab^2-b^3-(a^3+ab^2)$
		$y(b^2-a^2)=a^2b+2ab^2-b^3-a^3-ab^2$
		$y(b^2-a^2)=a^2b+ab^2-a^3-b^3$
		$y=\dfrac{a^2b+ab^2-a^3-b^3}{b^2-a^2}$
		$y=\dfrac{(ab)(a+b)-a^3-b^3}{(b+a)(b-a)}$
		$y=\dfrac{(ab)(a+b)+(-1)(a+b)(a^2-ab+b^2)}{(b+a)(b-a)}$
		$y=\dfrac{ab-a^2+ab-b^2}{(b-a)}$
		$y=\dfrac{(-1)(a^2-2ab+b^2)}{(b-a)}$
		$y=\dfrac{(-1)(a-b)(a-b)}{(b-a)}$
		$y=a-b$
		
		$bx+a(a-b)=a^2+b^2$
		$bx+a^2-ab=a^2+b^2$
		$bx=b^2+ab$
		$x=a+b$
5. For each of the following, eliminate $h$ and express $s$ in terms of $a$
	1. $s=ah$ and $h=2a+1$
		$h=\dfrac{s}{a}$
		$\dfrac{s}{a}=2a+1$
		$s=2a^2+a$
	1. $s=ah$ and $h=a(2+h)$
		$h=\dfrac{s}{a}$
		$\dfrac{s}{a}=2a+\dfrac{as}{a}$
		$\dfrac{s}{a}=2a+s$
		$\dfrac{s-sa}{a}=2a$
		$s(1-a)=2a^2$
		$s=\dfrac{2a^2}{1-a}$
	1. $s=h^2+ah$ and $h=3a^2$
		$s=9a^4+3a^3$
	1. $as=a+h$ and $h+ah=1$
		$h=\dfrac{1}{1+a}$
		$as=a+\dfrac{1}{1+a}$
		$s=1+\dfrac{1}{x^2+a}$
		$s=\dfrac{a^2+a+1}{a^2+a}$
	1. $as=s+h$ and $ah=a+h$
		$h=\dfrac{a}{a-1}$
		$as=s+\dfrac{a}{a-1}$
		$as-s=\dfrac{a}{a-1}$
		$s(a-1)=\dfrac{a}{a-1}$
		$s=\dfrac{a}{(a-1)^2}$
	1. $as=a+2h$ and $h=a-s$
		$h=\dfrac{as-a}{2}$
		$\dfrac{as-a}{2}=a-s$
		$as-a=2a-2s$
		$as+2s=3a$
		$s=\dfrac{3a}{a+2}$
